templates/flows/multiset_flows.v
@@ -3,16 +3,13 @@ Set Default Proof Using "All".
 Require Export flows ccm.
 Require Import Coq.Setoids.Setoid.
 
-(** Flow interface cameras and auxiliary lemmas for inset flows
-  (used in the give-up template proof). *)
+(** Flow interface cameras and auxiliary lemmas for multiset flows *)
 
 Section multiset_flows.
 
 Context `{Countable K}.
 
-(* Definition KS := @KS K _ _. *)
-
-(** CCM of multisets over keys *)
+(** CCM of finite multisets over a countable set K *)
 
 Definition K_multiset := nzmap K nat.
 
@@ -35,6 +32,9 @@ Definition in_inset k I n := k ∈ dom_ms (inf I n).
 Definition in_outset k I n := k ∈ dom_ms (out I n).
 
 Definition in_outsets k In := ∃ n, in_outset k In n.
+
+Definition closed I := ∀ k n, k ∉ outset I n.
+
 
 Lemma composable_outflow_leq_inflow I1 I2 k n :
   n ∈ domm I2 →
@@ -120,61 +120,123 @@ Proof.
   all: apply K_multiset_ccm.
 Qed.
 
-(** The following few definitions and lemmas can also be moved to ccm.v *)
-Definition nzmap_map (f : nat -> nat) (k: K) (m: nzmap K nat) : nzmap K nat :=
-  <<[ k := f (m ! k) ]>> m.
-
-Lemma nzmap_lookup_total_map f k m :
-      nzmap_map f k m ! k = f (m ! k).
+Lemma intComp_out_zero I1 I2 n : 
+        ✓ (I1 ⋅ I2) → n ∉ domm (I1 ⋅ I2) → out (I1 ⋅ I2) n = 0%CCM → out I2 n = 0%CCM.
 Proof.
-  unfold nzmap_map.
-  rewrite nzmap_lookup_total_insert.
+  intros Hvld Hn Hout. apply nzmap_eq. intros k.       
+  assert (out (I1 ⋅ I2) n = (out (I1) n) + (out I2 n))%CCM.
+  { apply intComp_unfold_out; try done. }
+  assert (out (I1 ⋅ I2) n ! k = (out (I1) n) ! k + (out I2 n) ! k)%CCM.
+  { rewrite H0. by rewrite lookup_op. }
+  rewrite Hout in H1. rewrite nzmap_lookup_empty in H1.
+  unfold ccmunit,ccm_unit in H1. simpl in H1.
+  unfold nat_unit in H1. unfold ccmop, nat_op in H1.
+  assert (out I2 n ! k = 0). lia.
+  rewrite H2. rewrite nzmap_lookup_empty. unfold ccmunit, ccm_unit. 
+  simpl. by unfold nat_unit.
+Qed. 
+
+Lemma flowint_step :
+  ∀ I I1 I2 k n,
+    ✓ I →
+    closed I →
+    I = I1 ⋅ I2 → k ∈ outset I1 n → n ∈ domm I2.
+Proof.
+  intros I I1 I2 k n vI cI dI kOut.
+  rewrite dI in vI.
+  
+  assert (domm I = domm I1 ∪ domm I2) as disj.
+  pose proof (intComp_dom _ _ vI).
+  rewrite dI.
   trivial.
+
+  (* First, prove n ∉ domm I1 *)
+  destruct (decide (n ∈ domm I1)).
+  pose proof (intComp_valid_proj1 I1 I2 vI) as vI1.
+  pose proof (intValid_in_dom_not_out I1 n vI1 e).
+  unfold outset, dom_ms in kOut.
+  rewrite nzmap_elem_of_dom_total in kOut *.
+  intros.
+  unfold ccmunit, ccm_unit, K_multiset_ccm, lift_ccm, lift_unit in H0.
+  rewrite H0 in H1.
+  rewrite nzmap_lookup_empty in H1.
+  contradiction.
+    
+  (* Now, prove n ∈ domm I *)    
+  assert (n ∈ domm (I1 ⋅ I2)) as in_Inf_n.
+  pose proof (intComp_unfold_out I1 I2 vI n).
+  destruct (decide (n ∉ domm (I1 ⋅ I2))).
+  apply H0 in n1.
+  pose proof (cI k n) as not_k_out.
+  unfold outset, dom_ms in not_k_out.
+  rewrite nzmap_elem_of_dom_total in not_k_out *.
+  intros not_k_out.
+  apply dec_stable in not_k_out.
+  unfold outset, dom_ms in kOut.
+  rewrite nzmap_elem_of_dom_total in kOut *.
+  intros kOut.
+  assert (out I n ! k = out (I1 ⋅ I2) n ! k).
+  rewrite dI. reflexivity.
+  rewrite n1 in H1.
+  rewrite lookup_op in H1.
+  unfold ccmop, ccm_op in H1.
+  unfold K_multiset_ccm,ccmunit,ccm_unit,nat_ccm,nat_unit,nat_op in kOut, not_k_out, H1.
+  lia.
+  apply dec_stable in n1. trivial.
+    
+  (* Finally, prove n ∈ domm I2 *)
+  apply intComp_dom in vI.
+  rewrite vI in in_Inf_n.
+  set_solver.
 Qed.
 
-Definition nzmap_map_set (f : nat -> nat) (s: gset K) (m : nzmap K nat) : nzmap K nat :=
-  let g := λ k m', nzmap_map f k m' in
-  set_fold g m s.
-
-
-Lemma nzmap_lookup_total_map_set_aux f s m :
-      ∀ k, (k ∈ s → nzmap_map_set f s m ! k = f (m ! k))
-         ∧ (k ∉ s → nzmap_map_set f s m ! k = m ! k).
+Lemma outset_distinct : ∀ I n, ✓ I ∧ (∃ k, k ∈ outset I n) → n ∉ domm I.
 Proof.
-    set (P := λ (m': nzmap K nat) (X: gset K),
-                    ∀ x, (x ∈ X → m' ! x = f (m ! x))
-                       ∧ (x ∉ X → m' ! x = m ! x) ).
-    apply (set_fold_ind_L P); try done.
-    intros x X r Hx HP.
-    unfold P in HP. unfold P.
-    intros x'.
-    destruct (decide (x' = x));
-      split; intros Hx'.
-    - rewrite e. rewrite nzmap_lookup_total_insert.
-      apply HP in Hx. by rewrite Hx.
-    - rewrite e in Hx'.
-      assert (x ∈ X). set_solver. contradiction.
-    - assert (x' ∈ X) as x'_in_X. set_solver.
-      apply HP in x'_in_X.
-      rewrite nzmap_lookup_total_insert_ne.
-      done. done.
-    - assert (x' ∉ X) as x'_nin_X. set_solver.
-      apply HP in x'_nin_X.
-      rewrite nzmap_lookup_total_insert_ne.
-      done. done.
+  intros.
+  destruct H0 as (VI & Out).
+  destruct Out as [k Out].
+
+  apply flowint_valid_unfold in VI.
+  destruct VI as (Ir & dI & disj & _).
+
+  rewrite (@map_disjoint_dom Node (gmap Node) (gset Node)) in disj *.
+  intros disj.
+
+  unfold outset, dom_ms, nzmap_dom, out, out_map in Out.
+  rewrite dI in Out.
+  rewrite nzmap_elem_of_dom_total in Out *.
+  intros Out.
+  destruct (decide (outR Ir ! n = ∅)).
+  rewrite e in Out.
+  rewrite nzmap_lookup_empty in Out.
+  contradiction.
+  rewrite <- nzmap_elem_of_dom_total in n0.
+  unfold dom, nzmap_dom in n0.
+  
+  unfold domm, dom, flowint_dom, inf_map.
+  rewrite dI.
+  set_solver.
 Qed.
 
-Lemma nzmap_lookup_total_map_set f k s m :
-      k ∈ s → nzmap_map_set f s m ! k = f (m ! k).
+Lemma flowint_inset_step : ∀ I1 I2 k n,
+    ✓ (I1 ⋅ I2) → n ∈ domm I2 → k ∈ outset I1 n → k ∈ inset I2 n.
 Proof.
-  apply nzmap_lookup_total_map_set_aux.
+  intros ? ? ? ? I12V Out Inset.
+  apply intComposable_valid in I12V.
+  pose proof (composable_outflow_leq_inflow I1 I2 k n Out I12V).
+  unfold outset, dom_ms in Inset.
+  rewrite nzmap_elem_of_dom_total in Inset *; intros Inset.
+  unfold inset, dom_ms.
+  rewrite nzmap_elem_of_dom_total.
+  unfold ccmunit, ccm_unit, nat_ccm, nat_unit in Inset.
+  unfold ccmunit, ccm_unit, nat_ccm, nat_unit.
+  assert (out I1 n ! k > 0 ∨ out I1 n ! k = 0). lia.
+  destruct H1.
+  assert (inf I2 n ! k ≠ 0). lia. trivial. contradiction.
 Qed.
 
-Lemma nzmap_lookup_total_map_set_ne f k s m :
-      k ∉ s → nzmap_map_set f s m ! k = m ! k.
-Proof.
-  apply nzmap_lookup_total_map_set_aux.
-Qed.
+
+(** The following few definitions and lemmas can also be moved to ccm.v *)
 
 Definition outflow_map_set f I (n: Node) (s: gset K) : multiset_flowint_ur := 
   let I_out_n := (nzmap_map_set f s (out I n)) in
@@ -919,181 +981,6 @@ Proof.
 Qed.
 
 
-Lemma flowint_step :
-  ∀ I I1 I2 k n root,
-    globalinv root I → I = I1 ⋅ I2 → k ∈ outset I1 n → n ∈ domm I2.
-Proof.
-  intros I I1 I2 k n r gInv dI kOut.
-  unfold globalinv in gInv.
-  destruct gInv as (vI & rI & cI & _).
-  rewrite dI in vI.
-  
-  assert (domm I = domm I1 ∪ domm I2) as disj.
-  pose proof (intComp_dom _ _ vI).
-  rewrite dI.
-  trivial.
-
-  (* First, prove n ∉ domm I1 *)
-  destruct (decide (n ∈ domm I1)).
-  pose proof (intComp_valid_proj1 I1 I2 vI) as vI1.
-  pose proof (intValid_in_dom_not_out I1 n vI1 e).
-  unfold outset, dom_ms in kOut.
-  rewrite nzmap_elem_of_dom_total in kOut *.
-  intros.
-  unfold ccmunit, ccm_unit, K_multiset_ccm, lift_ccm, lift_unit in H0.
-  rewrite H0 in H1.
-  rewrite nzmap_lookup_empty in H1.
-  contradiction.
-    
-  (* Now, prove n ∈ domm I *)    
-  assert (n ∈ domm (I1 ⋅ I2)) as in_Inf_n.
-  pose proof (intComp_unfold_out I1 I2 vI n).
-  destruct (decide (n ∉ domm (I1 ⋅ I2))).
-  apply H0 in n1.
-  pose proof (cI k n) as not_k_out.
-  unfold outset, dom_ms in not_k_out.
-  rewrite nzmap_elem_of_dom_total in not_k_out *.
-  intros not_k_out.
-  apply dec_stable in not_k_out.
-  unfold outset, dom_ms in kOut.
-  rewrite nzmap_elem_of_dom_total in kOut *.
-  intros kOut.
-  assert (out I n ! k = out (I1 ⋅ I2) n ! k).
-  rewrite dI. reflexivity.
-  rewrite n1 in H1.
-  rewrite lookup_op in H1.
-  unfold ccmop, ccm_op in H1.
-  unfold K_multiset_ccm,ccmunit,ccm_unit,nat_ccm,nat_unit,nat_op in kOut, not_k_out, H1.
-  lia.
-  apply dec_stable in n1. trivial.
-    
-  (* Finally, prove n ∈ domm I2 *)
-  apply intComp_dom in vI.
-  rewrite vI in in_Inf_n.
-  set_solver.
-Qed.
-
-Lemma outset_distinct : ∀ I n, ✓ I ∧ (∃ k, k ∈ outset I n) → n ∉ domm I.
-Proof.
-  intros.
-  destruct H0 as (VI & Out).
-  destruct Out as [k Out].
-
-  apply flowint_valid_unfold in VI.
-  destruct VI as (Ir & dI & disj & _).
-
-  rewrite (@map_disjoint_dom Node (gmap Node) (gset Node)) in disj *.
-  intros disj.
-
-  unfold outset, dom_ms, nzmap_dom, out, out_map in Out.
-  rewrite dI in Out.
-  rewrite nzmap_elem_of_dom_total in Out *.
-  intros Out.
-  destruct (decide (outR Ir ! n = ∅)).
-  rewrite e in Out.
-  rewrite nzmap_lookup_empty in Out.
-  contradiction.
-  rewrite <- nzmap_elem_of_dom_total in n0.
-  unfold dom, nzmap_dom in n0.
-  
-  unfold domm, dom, flowint_dom, inf_map.
-  rewrite dI.
-  set_solver.
-Qed.
-
-
-Lemma inset_monotone : ∀ I I1 I2 k n,
-    ✓ I → I = I1 ⋅ I2 → k ∈ inset I n → n ∈ domm I1 → k ∈ inset I1 n.
-Proof.
-  intros ? ? ? ? ? VI ID Inset Dom.
-  rewrite ID in VI.
-  pose proof (intComp_unfold_inf_1 I1 I2 VI n) as Inf1.
-  apply Inf1 in Dom.
-  assert (Inset1 := Inset).
-  unfold inset, dom_ms, nzmap_dom in Inset.
-  rewrite nzmap_elem_of_dom in Inset *.
-  intros Inset.
-  unfold inf, inf_map in Dom.
-  pose proof (intComp_valid_proj1 I1 I2 VI) as VI1.
-  apply flowint_valid_defined in VI1.
-  destruct VI1 as [I1r I1D].
-  pose proof (intComp_valid_proj2 I1 I2 VI) as VI2.
-  apply flowint_valid_defined in VI2.
-  destruct VI2 as [I2r I2D].
-
-  apply flowint_valid_defined in VI.
-  destruct VI as [I12r I12D].
-
-  rewrite I1D in Dom.
-  rewrite I1D in I12D.
-  rewrite I12D in Dom.
-
-  unfold inset, inf, dom_ms, inf_map.
-  rewrite I1D.
-  rewrite Dom.
-  rewrite nzmap_elem_of_dom_total.
-  rewrite lookup_op.
-  unfold nzmap_total_lookup.
-  unfold inf, is_Some, inf_map in Inset.
-  destruct Inset as [x Inset].
-  rewrite ID in Inset.
-  rewrite I1D in Inset.
-  rewrite I12D in Inset.
-  rewrite Inset.
-  simpl.
-  
-  assert (x <> 0).
-  unfold inset, dom_ms in Inset1.
-  rewrite nzmap_elem_of_dom_total in Inset1 *.
-  intros xDef.
-  rewrite ID in xDef.
-  rewrite I1D in xDef.
-  rewrite I12D in xDef.
-  unfold inf, inf_map in xDef.
-  unfold nzmap_total_lookup in xDef.
-  rewrite Inset in xDef.
-  simpl in xDef.
-  trivial.
-  
-  unfold ccmop, ccm_op, nat_ccm, nat_op, out, out_map.
-  unfold ccmunit, nat_unit.
-  lia.
-  all: apply K_multiset_ccm.
-Qed.
-
-Lemma flowint_inset_step : ∀ I1 I2 k n,
-    ✓ (I1 ⋅ I2) → n ∈ domm I2 → k ∈ outset I1 n → k ∈ inset I2 n.
-Proof.
-  intros ? ? ? ? I12V Out Inset.
-
-  pose proof (intComp_valid_proj1 I1 I2 I12V) as I1V.
-  pose proof (intComp_valid_proj2 I1 I2 I12V) as I2V.
-  apply flowint_valid_defined in I1V.
-  destruct I1V as [I1r I1Def].
-  apply flowint_valid_defined in I2V.
-  destruct I2V as [I2r I2Def].
-  pose proof (flowint_valid_defined _ _ I12V) as I12Def.
-  destruct I12Def as [I12r I12Def].
-
-  pose proof (intComp_unfold_inf_2 I1 I2 I12V n Out) as Inf2.
-
-  unfold outset in Inset.
-  unfold inset, dom_ms.
-  rewrite Inf2.
-  unfold out, out_map.
-  rewrite I1Def.
-  repeat rewrite nzmap_elem_of_dom_total.
-  repeat rewrite lookup_op.
-
-  unfold dom_ms, out, out_map in Inset.
-  rewrite I1Def in Inset.
-  repeat (rewrite nzmap_elem_of_dom_total in Inset *; intros Inset).
-  unfold ccmop, ccm_op, nat_ccm, nat_op.
-  unfold ccmop, ccm_op, nat_ccm, nat_op in Inset.
-  unfold ccmunit, ccm_unit, nat_unit, K_multiset_ccm, prod_ccm.
-  unfold ccmunit, ccm_unit, nat_unit, K_multiset_ccm, prod_ccm in Inset.
-  lia.
-Qed.
 
 Lemma contextualLeq_impl_globalinv : ∀ I I' root,
     globalinv root I →
@@ -1161,21 +1048,6 @@ Proof.
   set_solver.
 Qed.
 
-Lemma intComp_out_zero I1 I2 n : 
-        ✓ (I1 ⋅ I2) → n ∉ domm (I1 ⋅ I2) → out (I1 ⋅ I2) n = 0%CCM → out I2 n = 0%CCM.
-Proof.
-  intros Hvld Hn Hout. apply nzmap_eq. intros k.       
-  assert (out (I1 ⋅ I2) n = (out (I1) n) + (out I2 n))%CCM.
-  { apply intComp_unfold_out; try done. }
-  assert (out (I1 ⋅ I2) n ! k = (out (I1) n) ! k + (out I2 n) ! k)%CCM.
-  { rewrite H0. by rewrite lookup_op. }
-  rewrite Hout in H1. rewrite nzmap_lookup_empty in H1.
-  unfold ccmunit,ccm_unit in H1. simpl in H1.
-  unfold nat_unit in H1. unfold ccmop, nat_op in H1.
-  assert (out I2 n ! k = 0). lia.
-  rewrite H2. rewrite nzmap_lookup_empty. unfold ccmunit, ccm_unit. 
-  simpl. by unfold nat_unit.
-Qed. 
 *)
 End multiset_flows.
 
@@ -1185,4 +1057,4 @@ Arguments outset _ {_ _} _ _ : assert.
 Arguments in_inset _ {_ _} _ _ _ : assert.
 Arguments in_outset _ {_ _} _ _ _ : assert.
 Arguments in_outsets _ {_ _} _ _ : assert.
-(*Arguments globalinv _ {_ _} _ _ : assert.*)
+Arguments closed _ {_ _} _ : assert.
