templates/single_copy/link.v
@@ -20,8 +20,8 @@ Section Link_Cameras.
 
   (* RA for authoritative flow interfaces over pairs of multisets of keys *)
   Class flowintG Σ :=
-    FlowintG { flowint_inG :> inG Σ (authR (inset_flowint_ur K)) }.
-  Definition flowintΣ : gFunctors := #[GFunctor (authR (inset_flowint_ur K))].
+    FlowintG { flowint_inG :> inG Σ (authR (multiset_flowint_ur K)) }.
+  Definition flowintΣ : gFunctors := #[GFunctor (authR (multiset_flowint_ur K))].
 
   Instance subG_flowintΣ {Σ} : subG flowintΣ Σ → flowintG Σ.
   Proof. solve_inG. Qed.
@@ -45,8 +45,8 @@ Section Link_Cameras.
 
   (* RA for fractional interfaces *)
   Class fracintG Σ :=
-    FracinthG { fracint_inG :> inG Σ (authR (inset_flowint_ur K)) }.
-  Definition fracintΣ : gFunctors := #[GFunctor (authR (inset_flowint_ur K))].
+    FracinthG { fracint_inG :> inG Σ (authR (multiset_flowint_ur K)) }.
+  Definition fracintΣ : gFunctors := #[GFunctor (authR (multiset_flowint_ur K))].
 
   Instance subG_fracintΣ {Σ} : subG fracintΣ Σ → fracintG Σ.
   Proof. solve_inG. Qed.
@@ -90,7 +90,7 @@ Section Link_Template.
 
   (* The node predicate is specific to each template implementation. See GRASShopper files
      b-link.spl and hashtbl-link.spl for the concrete definitions. *)
-  Parameter node : Node → inset_flowint_ur K → gset K → iProp.
+  Parameter node : Node → multiset_flowint_ur K → gset K → iProp.
 
   (* The following assumption is justified by the fact that GRASShopper uses a
    * first-order separation logic. *)
@@ -109,7 +109,7 @@ Section Link_Template.
   (* The following specs are proved for each implementation in GRASShopper
    * (see b-link.spl and hashtbl-link.spl *)
 
-  Parameter findNext_spec : ∀ (n: Node) (k: K) (In : inset_flowint_ur K) (C: gset K),
+  Parameter findNext_spec : ∀ (n: Node) (k: K) (In : multiset_flowint_ur K) (C: gset K),
     ⊢ ({{{ ⌜k ∈ KS⌝ ∗ node n In C ∗ ⌜in_inset K k In n⌝ }}}
          findNext #n #k
        {{{ (succ: bool) (np: Node),
@@ -119,7 +119,7 @@ Section Link_Template.
                           | false => ⌜¬in_outsets K k In⌝ end) }}})%I.
 
   Parameter decisiveOp_spec : ∀ (dop: dOp) (n: Node) (k: K)
-      (In: inset_flowint_ur K) (C: gset K),
+      (In: multiset_flowint_ur K) (C: gset K),
     ⊢ ({{{ ⌜k ∈ KS⌝ ∗ node n In C ∗ ⌜in_inset K k In n⌝ ∗ ⌜¬in_outsets K k In⌝ }}}
          decisiveOp dop #n #k
        {{{ (succ: bool) (res: bool) (C1: gset K),
@@ -150,7 +150,7 @@ Section Link_Template.
     ∗ own (γ_i n) (● (inset K In n)).
 
   Definition nodeFull γ_I γ_f γ_k γ_i γ_h n : iProp :=
-    (∃ (b: bool) (In: inset_flowint_ur K),
+    (∃ (b: bool) (In: multiset_flowint_ur K),
         lockLoc n ↦ #b
         ∗ (if b then True else (∃ Cn, nodePred γ_f γ_h γ_k n In Cn))
         ∗ nodeShared γ_I γ_i γ_h n In).
@@ -322,7 +322,11 @@ Section Link_Template.
     iPoseProof (own_valid with "HI") as "%".
     iPoseProof (own_valid with "HIn") as "%".
     (* Prove the preconditions of ghost_snapshot_fp *)
-    assert (n' ∈ domm Io). by eauto using flowint_step.
+    assert (n' ∈ domm Io). 
+    { apply (flowint_step I In Io k); try done.
+        by rewrite auth_auth_valid in H5 *.
+        unfold globalinv in H3. destruct H3 as (_ & _ & cI & _). done.
+    }
     assert (domm I = domm In ∪ domm Io). {
       rewrite incl. rewrite flowint_comp_fp. done.
       rewrite <- incl. by apply auth_auth_valid.
@@ -470,7 +474,7 @@ Section Link_Template.
     ⊢ ⌜k ∈ KS⌝ -∗ inFP γ_f n -∗ inInr γ_i k n -∗
         <<< ∀ C, CSS γ_I γ_f γ_k γ_i γ_h r C >>>
             traverse #n #k @ ⊤
-        <<< ∃ (n': Node) (In': inset_flowint_ur K) (Cn': gset K),
+        <<< ∃ (n': Node) (In': multiset_flowint_ur K) (Cn': gset K),
             CSS γ_I γ_f γ_k γ_i γ_h r C
             ∗ nodePred γ_f γ_h γ_k n' In' Cn'
             ∗ ⌜in_inset K k In' n'⌝ ∗ ⌜¬in_outsets K k In'⌝,
